LiveVerif/src/LiveVerifExamples/mbuf.v
@@ -5,16 +5,24 @@ Load LiveVerif.
 
 Definition MBUF_SIZE := 2048.
 
+(* Note: this will result in mbufs slightly bigger than half of a 4KB page,
+   so most mbufs will span two pages, which seems bad --> don't do this!
 Record mbuf_t := {
   mbuf_len: Z;
   mbuf_data: list Z;
 }.
-
 Definition mbuf(r: mbuf_t): word -> mem -> Prop := .**/
   typedef struct __attribute__ ((__packed__)) {
     size_t mbuf_len;
     uint8_t mbuf_data[MBUF_SIZE];
-  } mbuf_t;
-/**.
+  } mbuf;
+/**. *)
+
+Definition mbuf(n: Z)(bs: list Z)(a: word): mem -> Prop :=
+  <{ * array (uint 8) n bs a
+     * array (uint 8) (MBUF_SIZE - n) ? (a ^+ /[n]) }>.
 
 End LiveVerif.
+
+#[export] Hint Extern 1 (PredicateSize (mbuf ?n ?bs)) => exact MBUF_SIZE
+: typeclass_instances.
